Util.v
@@ -19,3 +19,13 @@ Proof.
   intros. unfold decidable. eauto using excluded_middle.
 Qed.
 
+(* dec *)
+
+From Coq Require Arith.Compare_dec.
+From Coq Require Arith.Peano_dec.
+From Coq Require Strings.String.
+
+Definition nat_eq_dec := Peano_dec.eq_nat_dec.
+Definition string_eq_dec := String.string_dec.
+Definition lt_eq_lt_dec := Compare_dec.lt_eq_lt_dec.
+
