CoreExt.v
@@ -1,0 +1,232 @@
+From Coq Require Import Lia.
+
+From Elo Require Import Util.
+From Elo Require Import Array.
+From Elo Require Import Map.
+From Elo Require Import Core.
+
+(* ------------------------------------------------------------------------- *)
+(* dec                                                                       *)
+(* ------------------------------------------------------------------------- *)
+
+Theorem ityp_eq_dec : forall (T1 T2 : ityp),
+  {T1 = T2} + {T1 <> T2}.
+Proof. intros. decide equality; eauto. Qed.
+
+Theorem typ_eq_dec : forall (T1 T2 : typ),
+  {T1 = T2} + {T1 <> T2}.
+Proof. intros. decide equality; eauto using ityp_eq_dec. Qed.
+
+Theorem tm_eq_dec : forall (t1 t2 : tm),
+  {t1 = t2} + {t1 <> t2}.
+Proof.
+  intros. decide equality; eauto using nat_eq_dec, string_eq_dec, typ_eq_dec.
+Qed.
+
+Theorem effect_eq_dec : forall (e1 e2 : effect),
+  {e1 = e2} + {e1 <> e2}.
+Proof.
+  intros. decide equality; eauto using nat_eq_dec, typ_eq_dec, tm_eq_dec.
+Qed.
+
+(* ------------------------------------------------------------------------- *)
+(* array properties                                                          *)
+(* ------------------------------------------------------------------------- *)
+
+Definition forall_memory (m : mem) (P : tm -> _) : Prop :=
+  forall_array memory_default (fun tT => P (fst tT)) m.
+
+Definition forall_threads (ths : threads) (P : tm -> _) : Prop :=
+  forall_array thread_default P ths.
+
+Definition forall_program (m : mem) (ths : threads) (P : tm -> _) : Prop :=
+  (forall_memory m P) /\ (forall_threads ths P).
+
+#[export] Hint Unfold forall_program : core.
+
+Definition well_typed (t : tm) := exists T, empty |-- t is T.
+
+(* ------------------------------------------------------------------------- *)
+(* determinism                                                               *)
+(* ------------------------------------------------------------------------- *)
+
+Lemma deterministic_typing : forall Gamma t T1 T2,
+  Gamma |-- t is T1 ->
+  Gamma |-- t is T2 ->
+  T1 = T2.
+Proof.
+  intros * Htype1. generalize dependent T2.
+  induction Htype1; intros ? Htype2;
+  inversion Htype2; subst; eauto;
+  repeat match goal with
+  | IH : forall _, _ |-- ?t is _ -> _, H : _ |-- ?t is _ |- _ =>
+    eapply IH in H; subst
+  end;
+  congruence.
+Qed.
+
+Ltac apply_deterministic_typing :=
+  match goal with
+  | H1 : _ |-- ?t is ?T1, H2 : _ |-- ?t is ?T2 |- _ =>
+    assert (Heq : T1 = T2) by eauto using deterministic_typing; subst;
+    try (inversion Heq; subst; clear Heq)
+  end.
+
+(* ------------------------------------------------------------------------- *)
+(* auxiliary tactics                                                         *)
+(* ------------------------------------------------------------------------- *)
+
+Ltac induction_step :=
+  match goal with
+  | H : _ --[?e]--> _ |- _ =>
+    remember e as eff; induction H; inversion Heqeff; subst
+  end.
+
+Ltac inversion_step :=
+  match goal with
+  | H : _ --[_]--> _ |- _ => inversion H; subst; clear H
+  end.
+
+Ltac inversion_mstep :=
+  match goal with
+  | H : _ / _ ==[_]==> _ / _ |- _ => inversion H; subst
+  end.
+
+Ltac inversion_clear_mstep :=
+  match goal with
+  | H : _ / _ ==[_]==> _ / _ |- _ => inversion_subst_clear H
+  end.
+
+Ltac inversion_cstep :=
+  match goal with
+  | H : _ / _ ~~[_, _]~~> _ / _ |- _ => inversion H; subst
+  end.
+
+Ltac inversion_clear_cstep :=
+  match goal with
+  | H : _ / _ ~~[_, _]~~> _ / _ |- _ => inversion_subst_clear H
+  end.
+
+Ltac induction_multistep :=
+  match goal with
+  | H : _ / _ ~~[_]~~>* _ / _ |- _ => induction H
+  end.
+
+Ltac inversion_multistep :=
+  match goal with
+  | H : _ / _ ~~[_]~~>* _ / _ |- _ => inversion H; subst
+  end.
+
+Ltac inversion_clear_multistep :=
+  match goal with
+  | H : _ / _ ~~[_]~~>* _ / _ |- _ => inversion_subst_clear H
+  end.
+
+Ltac induction_type :=
+  match goal with
+  | H : _ |-- _ is _ |- _ => induction H
+  end.
+
+Ltac inversion_type :=
+  match goal with
+  | H : _ |-- <{ unit         }> is _ |- _ => inversion H; subst
+  | H : _ |-- <{ N _          }> is _ |- _ => inversion H; subst
+  | H : _ |-- <{ & _ :: _     }> is _ |- _ => inversion H; subst
+  | H : _ |-- <{ new _ _      }> is _ |- _ => inversion H; subst
+  | H : _ |-- <{ * _          }> is _ |- _ => inversion H; subst
+  | H : _ |-- <{ _ = _        }> is _ |- _ => inversion H; subst
+  | H : _ |-- <{ var _        }> is _ |- _ => inversion H; subst
+  | H : _ |-- <{ fn _ _ --> _ }> is _ |- _ => inversion H; subst
+  | H : _ |-- <{ call _ _     }> is _ |- _ => inversion H; subst
+  | H : _ |-- <{ _ ; _        }> is _ |- _ => inversion H; subst
+  | H : _ |-- <{ spawn _      }> is _ |- _ => inversion H; subst
+  end.
+
+Ltac inversion_clear_type :=
+  match goal with
+  | H : _ |-- <{ unit         }> is _ |- _ => inversion_subst_clear H
+  | H : _ |-- <{ N _          }> is _ |- _ => inversion_subst_clear H
+  | H : _ |-- <{ & _ :: _     }> is _ |- _ => inversion_subst_clear H
+  | H : _ |-- <{ new _ _      }> is _ |- _ => inversion_subst_clear H
+  | H : _ |-- <{ * _          }> is _ |- _ => inversion_subst_clear H
+  | H : _ |-- <{ _ = _        }> is _ |- _ => inversion_subst_clear H
+  | H : _ |-- <{ var _        }> is _ |- _ => inversion_subst_clear H
+  | H : _ |-- <{ fn _ _ --> _ }> is _ |- _ => inversion_subst_clear H
+  | H : _ |-- <{ call _ _     }> is _ |- _ => inversion_subst_clear H
+  | H : _ |-- <{ _ ; _        }> is _ |- _ => inversion_subst_clear H
+  | H : _ |-- <{ spawn _      }> is _ |- _ => inversion_subst_clear H
+  end.
+
+(* ------------------------------------------------------------------------- *)
+(* auxiliary lemmas                                                          *)
+(* ------------------------------------------------------------------------- *)
+
+Lemma step_length_tid : forall t ths tid e,
+  ths[tid] --[e]--> t ->
+  tid < #ths.
+Proof.
+  intros. decompose sum (lt_eq_lt_dec tid (#ths)); subst; trivial;
+  simpl_array; try lia; inversion_step.
+Qed.
+
+Corollary mstep_length_tid : forall m m' t' ths tid e,
+  m / ths[tid] ==[e]==> m' / t' ->
+  tid < #ths.
+Proof.
+  intros. inversion_mstep; eauto using step_length_tid.
+Qed.
+
+Corollary cstep_length_tid : forall m m' ths ths' tid e,
+  m / ths ~~[tid, e]~~> m' / ths' ->
+  tid < #ths.
+Proof.
+  intros. inversion_cstep; trivial.
+Qed.
+
+(* ------------------------------------------------------------------------- *)
+(* meta                                                                      *)
+(* ------------------------------------------------------------------------- *)
+
+Lemma cstep_preservation :
+  forall (P : mem -> tm -> Prop) m m' ths ths' tid e,
+    (* Memory step preserves the property. *)
+    (forall tid' t',
+      m / ths[tid'] ==[e]==> m' / t' ->
+      P m' t'
+    ) ->
+    (* The untouched threads and the new memory still preserve the property. *)
+    (forall tid' t',
+      tid <> tid' ->
+      tid' < #ths ->
+      m / ths[tid] ==[e]==> m' / t' ->
+      P m' ths[tid']
+    ) ->
+    (* The new thread preserves the property. *)
+    (forall block t',
+      ths[tid] --[EF_Spawn block]--> t' ->
+      P m block
+    ) ->
+    (* The term after the spawn preserves the property. *)
+    (forall block t',
+      ths[tid] --[EF_Spawn block]--> t' ->
+      P m t' 
+    ) ->
+    (* Unit preserves the property. *)
+    P m' thread_default ->
+    (* What we want to prove. *)
+    forall_threads ths (P m) ->
+    m / ths ~~[tid, e]~~> m' / ths' ->
+    forall_threads ths' (P m').
+Proof.
+  intros. inversion_cstep; intros tid'.
+  - destruct (nat_eq_dec tid' (#ths)); subst.
+    + rewrite <- (set_preserves_length _ tid t'). simpl_array. eauto.
+    + destruct (lt_eq_lt_dec tid' (length ths)) as [[Ha | ?] | Hb]; subst;
+      try lia.
+      * rewrite <- (set_preserves_length _ tid t') in Ha. simpl_array.
+        destruct (nat_eq_dec tid tid'); subst; simpl_array; eauto.
+      * rewrite <- (set_preserves_length _ tid t') in Hb. simpl_array. eauto.
+  - destruct (nat_eq_dec tid tid'); subst; simpl_array; eauto.
+    decompose sum (lt_eq_lt_dec tid' (#ths)); subst; eauto;
+    simpl_array; eauto.
+Qed.
