Soundness.v
@@ -7,6 +7,7 @@ From Elo Require Import Util.
 From Elo Require Import Array.
 From Elo Require Import Map.
 From Elo Require Import Core.
+From Elo Require Import CoreExt.
 From Elo Require Import ValidAddresses.
 From Elo Require Import Access.
 From Elo Require Import References.
